NuLLReps.thy
@@ -532,9 +532,9 @@ lemma [\<nu>intro]: "\<nu>Zero N z1 \<Longrightarrow> \<nu>Zero M z2 \<Longright
 lemma [\<nu>intro]: "\<^bold>c\<^bold>a\<^bold>s\<^bold>t x \<tycolon> N \<longmapsto> x' \<tycolon> N' \<^bold>m\<^bold>e\<^bold>a\<^bold>n\<^bold>w\<^bold>h\<^bold>i\<^bold>l\<^bold>e P \<Longrightarrow> \<^bold>c\<^bold>a\<^bold>s\<^bold>t y \<tycolon> M \<longmapsto> y' \<tycolon> M' \<^bold>m\<^bold>e\<^bold>a\<^bold>n\<^bold>w\<^bold>h\<^bold>i\<^bold>l\<^bold>e Q \<Longrightarrow>
   \<^bold>c\<^bold>a\<^bold>s\<^bold>t (x,y) \<tycolon> N \<nuFusion> M \<longmapsto> (x',y') \<tycolon> N' \<nuFusion> M' \<^bold>m\<^bold>e\<^bold>a\<^bold>n\<^bold>w\<^bold>h\<^bold>i\<^bold>l\<^bold>e P \<and> Q" unfolding Cast_def by auto
 
-abbreviation AutoFusion (infixr "\<nuFusion>''" 70)  where "N \<nuFusion>' M \<equiv> SchemaTag (N \<nuFusion> M)"
+definition AutoFusion (infixr "\<nuFusion>''" 70)  where "AutoFusion = Fusion"
 lemma [\<nu>intro]: "\<^bold>c\<^bold>a\<^bold>s\<^bold>t x \<tycolon> N \<nuFusion> M \<longmapsto> x' \<tycolon> N' \<nuFusion> M' \<^bold>m\<^bold>e\<^bold>a\<^bold>n\<^bold>w\<^bold>h\<^bold>i\<^bold>l\<^bold>e P \<Longrightarrow> \<^bold>c\<^bold>a\<^bold>s\<^bold>t x \<tycolon> N \<nuFusion> M \<longmapsto> x' \<tycolon> N' \<nuFusion>' M' \<^bold>m\<^bold>e\<^bold>a\<^bold>n\<^bold>w\<^bold>h\<^bold>i\<^bold>l\<^bold>e P"
-  unfolding Cast_def SchemaTag_def .
+  unfolding Cast_def AutoFusion_def .
 
 section \<open>Tuple\<close>
 
