NuBasicAbstractors.thy
@@ -1,7 +1,6 @@
 theory NuBasicAbstractors
   imports NuLLReps NuSys
-  abbrevs "<where>" = "\<^bold>w\<^bold>h\<^bold>e\<^bold>r\<^bold>e"
-    and "<some>" = "\<^bold>s\<^bold>o\<^bold>m\<^bold>e"
+  abbrevs "<some>" = "\<^bold>s\<^bold>o\<^bold>m\<^bold>e"
 begin
 
 \<nu>cast_overloads singular and plural
@@ -34,8 +33,9 @@ notation NuRefine (infixl "<where>" 80) and NuRefine (infixl "\<^bold>w\<^bold>h
 lemma [simp]: "p \<nuLinkL> N \<nuRefine> P \<nuLinkR> x \<longleftrightarrow> x \<in> P \<and> (p \<nuLinkL> N \<nuLinkR> x)" unfolding NuRefine_def Refining_ex by auto
 lemma [elim,\<nu>elim]: "x \<ratio> N \<nuRefine> P \<Longrightarrow> (x \<in> P \<Longrightarrow> x \<ratio> N \<Longrightarrow> C) \<Longrightarrow> C" unfolding Inhabited_def by auto
 lemma [\<nu>intro]: "(x \<in> P \<Longrightarrow> \<^bold>c\<^bold>a\<^bold>s\<^bold>t x \<tycolon> N \<longmapsto> Y \<^bold>m\<^bold>e\<^bold>a\<^bold>n\<^bold>w\<^bold>h\<^bold>i\<^bold>l\<^bold>e Q) \<Longrightarrow> \<^bold>c\<^bold>a\<^bold>s\<^bold>t x \<tycolon> N \<nuRefine> P \<longmapsto> Y \<^bold>m\<^bold>e\<^bold>a\<^bold>n\<^bold>w\<^bold>h\<^bold>i\<^bold>l\<^bold>e Q \<and>x \<in> P" unfolding Cast_def by auto
+lemma [\<nu>intro]: "\<^bold>c\<^bold>a\<^bold>s\<^bold>t x \<tycolon> N \<longmapsto> y \<tycolon> M \<^bold>m\<^bold>e\<^bold>a\<^bold>n\<^bold>w\<^bold>h\<^bold>i\<^bold>l\<^bold>e Q \<Longrightarrow> \<^bold>p\<^bold>r\<^bold>e\<^bold>m\<^bold>i\<^bold>s\<^bold>e y \<in> P \<Longrightarrow> \<^bold>c\<^bold>a\<^bold>s\<^bold>t x \<tycolon> N \<longmapsto> y \<tycolon> M <where> P \<^bold>m\<^bold>e\<^bold>a\<^bold>n\<^bold>w\<^bold>h\<^bold>i\<^bold>l\<^bold>e Q" unfolding Cast_def by auto
 lemma [\<nu>cast_overload E]: "\<^bold>c\<^bold>a\<^bold>s\<^bold>t x \<tycolon> (N \<^bold>w\<^bold>h\<^bold>e\<^bold>r\<^bold>e P) \<longmapsto> x \<tycolon> N \<^bold>m\<^bold>e\<^bold>a\<^bold>n\<^bold>w\<^bold>h\<^bold>i\<^bold>l\<^bold>e x \<in> P" unfolding Cast_def by auto
-lemma where_\<nu>cast: "\<^bold>p\<^bold>a\<^bold>r\<^bold>a\<^bold>m P \<Longrightarrow> \<^bold>p\<^bold>r\<^bold>e\<^bold>m\<^bold>i\<^bold>s\<^bold>e x \<in> P \<Longrightarrow> \<^bold>c\<^bold>a\<^bold>s\<^bold>t x \<tycolon> N \<longmapsto> x \<tycolon> (N \<^bold>w\<^bold>h\<^bold>e\<^bold>r\<^bold>e P)" unfolding Cast_def by auto
+lemma refine_\<nu>cast: "\<^bold>p\<^bold>a\<^bold>r\<^bold>a\<^bold>m P \<Longrightarrow> \<^bold>p\<^bold>r\<^bold>e\<^bold>m\<^bold>i\<^bold>s\<^bold>e x \<in> P \<Longrightarrow> \<^bold>c\<^bold>a\<^bold>s\<^bold>t x \<tycolon> N \<longmapsto> x \<tycolon> (N \<^bold>w\<^bold>h\<^bold>e\<^bold>r\<^bold>e P)" unfolding Cast_def by auto
 
 lemma [\<nu>intro]: "\<^bold>p\<^bold>r\<^bold>e\<^bold>m\<^bold>i\<^bold>s\<^bold>e \<forall>x. P' x \<longrightarrow> P x \<Longrightarrow> \<^bold>p\<^bold>r\<^bold>e\<^bold>m\<^bold>i\<^bold>s\<^bold>e \<forall>x z. P' x \<and> x \<in> S \<and> (x \<ratio> N) \<longrightarrow> s z x \<in> S \<Longrightarrow> \<nu>Share N P s \<Longrightarrow> \<nu>Share (N \<^bold>w\<^bold>h\<^bold>e\<^bold>r\<^bold>e S) P' s"
   unfolding \<nu>Share_def by (auto 0 3)
@@ -50,6 +50,7 @@ lemma [\<nu>intro]: "\<^bold>p\<^bold>r\<^bold>e\<^bold>m\<^bold>i\<^bold>s\<^bo
 definition SchemaCondition (infixl "<where''>" 80) where "SchemaCondition = NuRefine"
 
 lemma [simp]: "\<tort_lbrace>x \<tycolon> N <where'> P\<tort_rbrace> = (\<tort_lbrace>x \<tycolon> N\<tort_rbrace> \<addition> (x \<in> P))" unfolding SchemaCondition_def by auto
+lemma [\<nu>intro]: "\<^bold>c\<^bold>a\<^bold>s\<^bold>t x \<tycolon> N \<longmapsto> y \<tycolon> M <where> P \<^bold>m\<^bold>e\<^bold>a\<^bold>n\<^bold>w\<^bold>h\<^bold>i\<^bold>l\<^bold>e Q \<Longrightarrow> \<^bold>c\<^bold>a\<^bold>s\<^bold>t x \<tycolon> N \<longmapsto> y \<tycolon> M <where'> P \<^bold>m\<^bold>e\<^bold>a\<^bold>n\<^bold>w\<^bold>h\<^bold>i\<^bold>l\<^bold>e Q" unfolding SchemaCondition_def . 
 lemma SchemaCondition_simp: "\<tort_lbrace> x \<tycolon> N <where'> P\<tort_rbrace> = \<tort_lbrace> x \<tycolon> N \<^bold>w\<^bold>h\<^bold>e\<^bold>r\<^bold>e P\<tort_rbrace>" unfolding SchemaCondition_def by auto
 
 subsubsection \<open>Down Lifting\<close>
@@ -68,8 +69,8 @@ lemma "\<down>lift_\<nu>cast": "\<^bold>p\<^bold>a\<^bold>r\<^bold>a\<^bold>m g 
 definition Schema (infixl "<schema>" 80) where "Schema = DownLift"
 lemma i_schema_\<nu>cast: "\<^bold>p\<^bold>a\<^bold>r\<^bold>a\<^bold>m g \<Longrightarrow> \<^bold>p\<^bold>r\<^bold>e\<^bold>m\<^bold>i\<^bold>s\<^bold>e g y = x \<Longrightarrow> \<^bold>c\<^bold>a\<^bold>s\<^bold>t x \<tycolon> N \<longmapsto> y \<tycolon> N <schema> g" unfolding Cast_def Schema_def by auto
 lemma [simp]: "\<tort_lbrace> x \<tycolon> N <schema> id \<tort_rbrace> = \<tort_lbrace> x \<tycolon> N \<tort_rbrace>" and [simp]: "\<tort_lbrace> (a,b) \<tycolon> N <schema> f \<tort_rbrace> = \<tort_lbrace> f (a,b) \<tycolon> N \<tort_rbrace>" unfolding Schema_def by auto
-lemma [\<nu>intro]: "\<^bold>c\<^bold>a\<^bold>s\<^bold>t x \<tycolon> N \<longmapsto> y1 \<tycolon> M \<^bold>m\<^bold>e\<^bold>a\<^bold>n\<^bold>w\<^bold>h\<^bold>i\<^bold>l\<^bold>e P \<Longrightarrow> \<^bold>p\<^bold>r\<^bold>e\<^bold>m\<^bold>i\<^bold>s\<^bold>e y1 = g y  \<Longrightarrow> \<^bold>c\<^bold>a\<^bold>s\<^bold>t x \<tycolon> N \<longmapsto> y \<tycolon> M <schema> g"
-  unfolding Schema_def Cast_def by auto
+lemma [\<nu>intro]: "\<^bold>c\<^bold>a\<^bold>s\<^bold>t x \<tycolon> N \<longmapsto> y1 \<tycolon> M \<^bold>m\<^bold>e\<^bold>a\<^bold>n\<^bold>w\<^bold>h\<^bold>i\<^bold>l\<^bold>e P \<Longrightarrow> <Structural> g y = y1  \<Longrightarrow> \<^bold>c\<^bold>a\<^bold>s\<^bold>t x \<tycolon> N \<longmapsto> y \<tycolon> M <schema> g"
+  unfolding Schema_def Cast_def StructuralTag_def by auto
 
 subsubsection \<open>Up Lifting\<close>
 
