NuPrim.thy
@@ -30,7 +30,6 @@ text \<open>The fundamental theory for \<nu>-system\<close>
 
 section Preliminary
 
-declare [[quick_and_dirty = true]]
 ML_file NuConfig.ML
 bundle show_more1 = [[show_hyps = true, show_types = true, show_sorts = true]]
 bundle show_more = [[show_hyps = true, show_types = true]]
@@ -402,8 +401,10 @@ instantiation prod :: (lrep,stack) stack begin instance by standard end
 
 definition Stack_Delimiter :: " ('a :: stack) set \<Rightarrow> ('b :: lrep) set \<Rightarrow> ('b \<times> 'a) set " ( "(2_/ \<heavy_comma> _)" [13,14] 13)
   where "Stack_Delimiter a b = (b \<times> a)"
-definition End_of_Contextual_Stack :: " 'a \<Rightarrow> 'a " ("\<^bold>E\<^bold>N\<^bold>D") where "End_of_Contextual_Stack x = x" \<comment> \<open>A tag for printing sugar\<close>
+definition End_of_Stack ("\<^bold>E\<^bold>N\<^bold>D") where "End_of_Stack = Void"
+definition End_of_Contextual_Stack :: " 'a \<Rightarrow> 'a " where "End_of_Contextual_Stack x = x" \<comment> \<open>A tag for printing sugar\<close>
 translations "a" <= "CONST End_of_Contextual_Stack x \<heavy_comma> a" \<comment> \<open>hide the end\<close>
+  "a" <= "CONST End_of_Stack\<heavy_comma> a"
 translations "R \<heavy_comma> x \<tycolon> N" == "R \<heavy_comma> \<tort_lbrace>x \<tycolon> N\<tort_rbrace>"
 lemma [elim,\<nu>elim]: "Inhabited (End_of_Contextual_Stack S) \<Longrightarrow> C \<Longrightarrow> C" .
 lemma [simp]: "(a,b) \<in> (B \<heavy_comma> A) \<longleftrightarrow> a \<in> A \<and> b \<in> B" unfolding Stack_Delimiter_def by simp
@@ -894,7 +895,7 @@ lemma CastI[intro]: "Inhabited A \<Longrightarrow> A \<subseteq> B \<Longrightar
   and [intro]: "\<not> Inhabited A \<Longrightarrow> \<^bold>c\<^bold>a\<^bold>s\<^bold>t A \<longmapsto> B \<^bold>m\<^bold>e\<^bold>a\<^bold>n\<^bold>w\<^bold>h\<^bold>i\<^bold>l\<^bold>e P" unfolding Cast_def Inhabited_def by auto
 lemma [\<nu>intro0]: "\<^bold>c\<^bold>a\<^bold>s\<^bold>t A \<longmapsto> A" by blast
 lemma "=_\<nu>cast": "\<^bold>p\<^bold>a\<^bold>r\<^bold>a\<^bold>m x' \<Longrightarrow> \<^bold>p\<^bold>r\<^bold>e\<^bold>m\<^bold>i\<^bold>s\<^bold>e x = x' \<Longrightarrow> \<^bold>c\<^bold>a\<^bold>s\<^bold>t x \<tycolon> N \<longmapsto> x' \<tycolon> N" unfolding Cast_def by auto
-lemma [\<nu>intro]: "\<^bold>p\<^bold>r\<^bold>e\<^bold>m\<^bold>i\<^bold>s\<^bold>e N = N' \<Longrightarrow> \<^bold>p\<^bold>r\<^bold>e\<^bold>m\<^bold>i\<^bold>s\<^bold>e x = x' \<Longrightarrow> \<^bold>c\<^bold>a\<^bold>s\<^bold>t \<tort_lbrace>x \<tycolon> N\<tort_rbrace> \<longmapsto> \<tort_lbrace>x' \<tycolon> N'\<tort_rbrace>" unfolding Cast_def Premise_def by simp
+lemma [\<nu>intro']: "\<^bold>p\<^bold>r\<^bold>e\<^bold>m\<^bold>i\<^bold>s\<^bold>e N = N' \<Longrightarrow> \<^bold>p\<^bold>r\<^bold>e\<^bold>m\<^bold>i\<^bold>s\<^bold>e x = x' \<Longrightarrow> \<^bold>c\<^bold>a\<^bold>s\<^bold>t \<tort_lbrace>x \<tycolon> N\<tort_rbrace> \<longmapsto> \<tort_lbrace>x' \<tycolon> N'\<tort_rbrace>" unfolding Cast_def Premise_def by simp
 lemma [\<nu>intro0]: "\<^bold>p\<^bold>r\<^bold>e\<^bold>m\<^bold>i\<^bold>s\<^bold>e x = x" unfolding Premise_def by simp
 lemma [\<nu>intro]: "\<^bold>c\<^bold>a\<^bold>s\<^bold>t A \<longmapsto> B \<^bold>m\<^bold>e\<^bold>a\<^bold>n\<^bold>w\<^bold>h\<^bold>i\<^bold>l\<^bold>e P \<Longrightarrow> \<^bold>c\<^bold>a\<^bold>s\<^bold>t \<S_S> A \<longmapsto> \<S_S> B \<^bold>m\<^bold>e\<^bold>a\<^bold>n\<^bold>w\<^bold>h\<^bold>i\<^bold>l\<^bold>e P" by blast
 lemma [\<nu>intro]: "\<^bold>c\<^bold>a\<^bold>s\<^bold>t A \<longmapsto> A' \<^bold>m\<^bold>e\<^bold>a\<^bold>n\<^bold>w\<^bold>h\<^bold>i\<^bold>l\<^bold>e P1 \<Longrightarrow> \<^bold>c\<^bold>a\<^bold>s\<^bold>t B \<longmapsto> B' \<^bold>m\<^bold>e\<^bold>a\<^bold>n\<^bold>w\<^bold>h\<^bold>i\<^bold>l\<^bold>e P2 \<Longrightarrow> \<^bold>c\<^bold>a\<^bold>s\<^bold>t (A\<heavy_comma>B) \<longmapsto> (A'\<heavy_comma>B') \<^bold>m\<^bold>e\<^bold>a\<^bold>n\<^bold>w\<^bold>h\<^bold>i\<^bold>l\<^bold>e P1 \<and> P2" by blast
@@ -905,6 +906,8 @@ lemma [\<nu>intro]: "\<^bold>c\<^bold>a\<^bold>s\<^bold>t A \<longmapsto> A' \<^
   unfolding Cast_def by auto
 
 theorem apply_cast: "(\<^bold>c\<^bold>u\<^bold>r\<^bold>r\<^bold>e\<^bold>n\<^bold>t blk \<^bold>r\<^bold>e\<^bold>s\<^bold>u\<^bold>l\<^bold>t\<^bold>s \<^bold>i\<^bold>n (R \<heavy_comma> X \<flower> W)) \<Longrightarrow> (\<^bold>c\<^bold>a\<^bold>s\<^bold>t X \<longmapsto> Y \<^bold>m\<^bold>e\<^bold>a\<^bold>n\<^bold>w\<^bold>h\<^bold>i\<^bold>l\<^bold>e P) \<Longrightarrow> (\<^bold>c\<^bold>u\<^bold>r\<^bold>r\<^bold>e\<^bold>n\<^bold>t blk \<^bold>r\<^bold>e\<^bold>s\<^bold>u\<^bold>l\<^bold>t\<^bold>s \<^bold>i\<^bold>n (R \<heavy_comma> Y \<flower> W) \<addition> P)"
+  unfolding Procedure_def CurrentConstruction_def PendingConstruction_def bind_def SpecTop_imp by (auto 4 6)
+theorem apply_cast': "(\<^bold>c\<^bold>u\<^bold>r\<^bold>r\<^bold>e\<^bold>n\<^bold>t blk \<^bold>r\<^bold>e\<^bold>s\<^bold>u\<^bold>l\<^bold>t\<^bold>s \<^bold>i\<^bold>n (R \<heavy_comma> X)) \<Longrightarrow> (\<^bold>c\<^bold>a\<^bold>s\<^bold>t X \<longmapsto> Y \<^bold>m\<^bold>e\<^bold>a\<^bold>n\<^bold>w\<^bold>h\<^bold>i\<^bold>l\<^bold>e P) \<Longrightarrow> (\<^bold>c\<^bold>u\<^bold>r\<^bold>r\<^bold>e\<^bold>n\<^bold>t blk \<^bold>r\<^bold>e\<^bold>s\<^bold>u\<^bold>l\<^bold>t\<^bold>s \<^bold>i\<^bold>n (R \<heavy_comma> Y) \<addition> P)"
   unfolding Procedure_def CurrentConstruction_def PendingConstruction_def bind_def SpecTop_imp by (auto 4 6)
 theorem cast: "\<^bold>c\<^bold>u\<^bold>r\<^bold>r\<^bold>e\<^bold>n\<^bold>t blk \<^bold>r\<^bold>e\<^bold>s\<^bold>u\<^bold>l\<^bold>t\<^bold>s \<^bold>i\<^bold>n T \<Longrightarrow> \<^bold>c\<^bold>a\<^bold>s\<^bold>t T \<longmapsto> T' \<^bold>m\<^bold>e\<^bold>a\<^bold>n\<^bold>w\<^bold>h\<^bold>i\<^bold>l\<^bold>e P \<Longrightarrow> \<^bold>c\<^bold>u\<^bold>r\<^bold>r\<^bold>e\<^bold>n\<^bold>t blk \<^bold>r\<^bold>e\<^bold>s\<^bold>u\<^bold>l\<^bold>t\<^bold>s \<^bold>i\<^bold>n T' "
   for T' :: "('a::lrep) set" unfolding Cast_def CurrentConstruction_def by auto
